template-coq/theories/Typing.v
@@ -1,6 +1,6 @@
 (* Distributed under the terms of the MIT license.   *)
 
-From Coq Require Import Bool String List Program BinPos Compare_dec Omega.
+From Coq Require Import Bool String List Program BinPos Compare_dec Arith Lia.
 From Template Require Import config utils Ast AstUtils univ Induction LiftSubst UnivSubst.
 From Template Require Loader.
 Require Import String.
@@ -1017,6 +1017,9 @@ Lemma on_type_lift_all `{checker_flags} P Σ Γ T :
   on_type (lift_typing P) Σ Γ T.
 Proof. intros. red in X, X0. red. red. destruct X. exists x.  apply X0. Qed.
 
+Lemma refine_type `{checker_flags} Σ Γ t T U : Σ ;;; Γ |- t : T -> T = U -> Σ ;;; Γ |- t : U.
+Proof. now intros Ht ->. Qed.
+
 Inductive Forall_typing_spine `{checker_flags} Σ Γ (P : term -> term -> Type) :
   forall (T : term) (t : list term) (U : term), typing_spine Σ Γ T t U -> Type :=
 | Forall_type_spine_nil T : Forall_typing_spine Σ Γ P T [] T (type_spine_nil Σ Γ T)
@@ -1082,8 +1085,6 @@ Proof.
   exact (S (Nat.max (wf_local_size _ typing_size _ a) (all_size _ (fun x p => typing_size Σ _ _ _ (fst p)) a0))).
   exact (S (Nat.max (wf_local_size _ typing_size _ a) (all_size _ (fun x p => typing_size Σ _ _ _ p) a0))).
 Defined.
-
-Require Import Lia.
 
 Lemma typing_size_pos `{checker_flags} {Σ Γ t T} (d : Σ ;;; Γ |- t : T) : typing_size d > 0.
 Proof.
@@ -1329,7 +1330,7 @@ Proof.
   inv wfΣ.
   constructor; auto. unfold Forall_decls_typing in IH.
   - specialize (IH (existT _ (Σ, φ) (existT _ X14 (existT _ [] (existT _ (localenv_nil typing (Σ, φ)) (existT _ (tSort Universe.type0m ) (existT _ _ (type_Sort _ _ Level.prop (localenv_nil typing (Σ, φ)))))))))).
-    simpl in IH. forward IH. constructor 1. simpl. omega.
+    simpl in IH. forward IH. constructor 1. simpl. lia.
     apply IH; auto.
   - simpl. simpl in *.
     (* specialize (IH (existT _ (Σ, φ) (existT _ X14 (existT _ [] (existT _ (localenv_nil typing (Σ, φ)) (existT _ (tSort Universe.type0m ) (existT _ _ (type_Sort _ _ Level.prop (localenv_nil typing (Σ, φ)))))))))). *)
@@ -1343,13 +1344,13 @@ Proof.
       intros. red in X15. simpl in X15.
       specialize (IH (existT _ (Σ, φ) (existT _ X14 (existT _ _ (existT _ (localenv_nil typing _) (existT _ _ (existT _ _ X15))))))).
       simpl in IH.
-      forward IH. constructor 1. simpl; omega.
+      forward IH. constructor 1. simpl; lia.
       apply IH.
       red. simpl. red in X15; simpl in X15.
       destruct X15 as [s Hs]. red. simpl. exists s.
       specialize (IH (existT _ (Σ, φ) (existT _ X14 (existT _ _ (existT _ (localenv_nil typing _) (existT _ _ (existT _ _ Hs))))))).
       simpl in IH.
-      forward IH. constructor 1. simpl; omega.
+      forward IH. constructor 1. simpl; lia.
       apply IH.
     + red in X15.
       destruct X15 as [onI onP onnp]; constructor; eauto.
@@ -1357,20 +1358,20 @@ Proof.
       constructor.
       ++ apply onArity in X15. destruct X15 as [[s Hs] Hpars]. split; auto. exists s.
          specialize (IH (existT _ (Σ, φ) (existT _ X14 (existT _ _ (existT _ (localenv_nil typing _) (existT _ _ (existT _ _ Hs))))))).
-         simpl in IH. apply IH; constructor 1; simpl; omega.
+         simpl in IH. apply IH; constructor 1; simpl; lia.
       ++ apply onConstructors in X15.
          red in X15 |- *. eapply Alli_impl; eauto. intros.
          red in X16 |- *. destruct X16 as [[s Hs] Hpars]. split; auto. exists s.
          pose proof (typing_wf_local (Σ:= (Σ, φ)) X14 Hs).
          specialize (IH (existT _ (Σ, φ) (existT _ X14 (existT _ _ (existT _ X16 (existT _ _ (existT _ _ Hs))))))).
-         simpl in IH. apply IH; constructor 1; simpl; omega.
+         simpl in IH. apply IH; constructor 1; simpl; lia.
       ++ apply onProjections in X15. simpl in *.
          red in X15 |- *. eapply Alli_impl; eauto. clear X15. intros.
          red in X15 |- *. destruct (decompose_prod_assum [] (ind_type x)).
          destruct X15 as [[s Hs] Hpars]. split; auto. exists s.
          pose proof (typing_wf_local (Σ:= (Σ, φ)) X14 Hs).
          specialize (IH (existT _ (Σ, φ) (existT _ X14 (existT _ _ (existT _ X15 (existT _ _ (existT _ _ Hs))))))).
-         simpl in IH. apply IH; constructor 1; simpl; omega.
+         simpl in IH. apply IH; constructor 1; simpl; lia.
       ++ red in onP |- *.
          eapply All_local_env_impl; eauto.
          intros. do 2 red in X15 |- *.
@@ -1567,87 +1568,24 @@ Proof.
          eapply (X _ X0 _ _ Hty). simpl; lia.
 Qed.
 
-(** Example: only well-formed terms are well-typed *)
+(** * Lemmas about All_local_env *)
 
-Lemma wf_mkApps_napp t u : isApp t = false -> Ast.wf (mkApps t u) -> Ast.wf t /\ List.Forall Ast.wf u.
+Definition on_local_decl (P : global_context -> context -> term -> term -> Type) Σ Γ d :=
+  match d.(decl_body) with
+  | Some b => P Σ Γ b d.(decl_type)
+  | None => { u & P Σ Γ d.(decl_type) (tSort u) }
+  end.
+
+Lemma nth_error_All_local_env {P Σ Γ n} (isdecl : n < #|Γ|) :
+  All_local_env P Σ Γ ->
+  on_some (on_local_decl P Σ (skipn (S n) Γ)) (nth_error Γ n).
 Proof.
-  induction u in t |- *; simpl.
-  - intuition.
-  - intros Happ H; destruct t; try solve [inv H; intuition auto].
-    specialize (IHu (tApp t (l ++ [a]))).
-    forward IHu.
-    induction u; trivial. discriminate.
-Qed.
-Hint Resolve wf_mkApps_napp : wf.
-
-Lemma wf_mkApps_inv t u : Ast.wf (mkApps t u) -> List.Forall Ast.wf u.
-Proof.
-  induction u in t |- *; simpl.
-  - intuition.
-  - intros H; destruct t; try solve [inv H; intuition auto].
-    specialize (IHu (tApp t (l ++ [a]))).
-    forward IHu.
-    induction u; trivial.
-    simpl. rewrite <- app_assoc. simpl. apply H.
-    intuition. inv H.
-    apply Forall_app in H3. intuition.
-Qed.
-Hint Resolve wf_mkApps_inv : wf.
-Hint Constructors Ast.wf : wf.
-
-Lemma isLambda_subst s t : isLambda t = true -> isLambda (subst0 s t) = true.
-Proof.
-  destruct t; simpl; try congruence.
-Qed.
-
-Lemma isLambda_isApp t : isLambda t = true -> isApp t = false.
-Proof. destruct t; simpl; congruence. Qed.
-
-Lemma unfold_fix_wf:
-  forall (mfix : mfixpoint term) (idx : nat) (narg : nat) (fn : term),
-    unfold_fix mfix idx = Some (narg, fn) ->
-    Ast.wf (tFix mfix idx) ->
-    Ast.wf fn /\ isApp fn <> true.
-Proof.
-  intros mfix idx narg fn Hf Hwf.
-  unfold unfold_fix in Hf. inv Hwf.
-  destruct nth_error eqn:eqnth; try congruence.
-  pose proof (nth_error_forall eqnth H). simpl in H0.
-  injection Hf. intros <- <-.
-  destruct H0 as [ _ [ wfd islamd ] ]. apply (isLambda_subst (fix_subst mfix)) in islamd.
-  apply isLambda_isApp in islamd. split; try congruence.
-  apply wf_subst; auto. clear wfd islamd Hf eqnth.
-  assert(forall n, Ast.wf (tFix mfix n)). constructor; auto.
-  unfold fix_subst. generalize #|mfix|; intros. induction n; auto.
-Qed.
-
-Lemma unfold_cofix_wf:
-  forall (mfix : mfixpoint term) (idx : nat) (narg : nat) (fn : term),
-    unfold_cofix mfix idx = Some (narg, fn) ->
-    Ast.wf (tCoFix mfix idx) -> Ast.wf fn.
-Proof.
-  intros mfix idx narg fn Hf Hwf.
-  unfold unfold_cofix in Hf. inv Hwf.
-  destruct nth_error eqn:eqnth; try congruence.
-  pose proof (nth_error_forall eqnth H). simpl in H0.
-  injection Hf. intros <- <-.
-  destruct H0 as [ _ wfd ].
-  apply wf_subst; auto. clear wfd Hf eqnth.
-  assert(forall n, Ast.wf (tCoFix mfix n)). constructor; auto.
-  unfold cofix_subst. generalize #|mfix|; intros. induction n; auto.
-Qed.
-
-Lemma wf_subst_instance_constr u c :
-  Ast.wf c -> Ast.wf (subst_instance_constr u c).
-Proof.
-  induction 1 using term_wf_forall_list_ind; simpl; try solve [ constructor; auto using Forall_map ].
-
-  constructor; auto. destruct t; simpl in *; try congruence. destruct l; simpl in *; congruence.
-  now apply Forall_map.
-  constructor; auto. merge_Forall. apply Forall_map.
-  eapply Forall_impl; eauto. intros. simpl in *. red. intuition auto.
-  destruct x; simpl in *.
-  destruct dbody; simpl in *; congruence.
+  induction 1 in n, isdecl |- *. red; simpl.
+  - destruct n; simpl; inv isdecl.
+  - destruct n. red; simpl. now exists u.
+    simpl. apply IHX. simpl in isdecl. lia.
+  - destruct n. auto.
+    apply IHX. simpl in *. lia.
 Qed.
 
 Lemma lookup_on_global_env P Σ c decl :
@@ -1661,58 +1599,6 @@ Proof.
   apply IHX.
 Qed.
 
-Lemma wf_nth:
-  forall (n : nat) (args : list term), Forall Ast.wf args -> Ast.wf (nth n args tDummy).
-Proof.
-  intros n args H. induction H in n; destruct n; simpl; try constructor; auto.
-Qed.
-Hint Resolve wf_nth.
-
-Lemma wf_red1 `{CF:checker_flags} Σ Γ M N :
-  on_global_env (fun Σ Γ t T => match t with Some b => Ast.wf b /\ Ast.wf T | None => Ast.wf T end) Σ ->
-  List.Forall (fun d => match decl_body d with Some b => Ast.wf b | None => True end) Γ ->
-  Ast.wf M -> red1 (fst Σ) Γ M N -> Ast.wf N.
-Proof.
-  intros wfΣ wfΓ wfM H.
-  induction H using red1_ind_all in wfM, wfΓ |- *; inv wfM; try solve[ constructor; auto with wf ].
-
-  - inv H1. inv H2.
-    eauto with wf.
-  - auto with wf.
-  - apply wf_lift.
-    unfold option_map in H. destruct nth_error eqn:Heq; try discriminate.
-    eapply nth_error_forall in wfΓ; eauto. simpl in *. destruct (decl_body c); congruence.
-  - unfold iota_red.
-    apply wf_mkApps_inv in H0.
-    apply wf_mkApps; auto.
-    induction brs in c, H1 |- *; destruct c; simpl in *. constructor. constructor.
-    inv H1; auto. inv H1; auto.
-    induction H0 in pars |- *; destruct pars; try constructor; auto. simpl. auto.
-  - apply unfold_fix_wf in H; auto. constructor; intuition auto.
-  - constructor; auto. apply wf_mkApps_napp in H1 as [Hcof Hargs]; auto.
-    apply unfold_cofix_wf in H; auto.
-    apply wf_mkApps; intuition auto.
-  - constructor; auto. apply wf_mkApps_napp in H0 as [Hcof Hargs]; auto.
-    apply unfold_cofix_wf in H; auto.
-    apply wf_mkApps; intuition auto.
-  - apply wf_subst_instance_constr.
-    unfold declared_constant in H.
-    eapply lookup_on_global_env in H as [Σ' [onΣ' prf]]; eauto.
-    destruct decl; simpl in *.
-    subst cst_body; intuition. red in prf. simpl in prf. easy.
-  - apply wf_mkApps_inv in H0.
-    eapply nth_error_forall in H0; eauto.
-  - constructor; auto. apply IHred1; auto. constructor; simpl; auto.
-  - constructor; auto. apply IHred1; auto. constructor; simpl; auto.
-  - constructor; auto. induction H; constructor; inv H2; intuition auto.
-  - apply wf_mkApps; auto.
-  - constructor; auto. induction H; congruence.
-    clear H1. induction H; inv H3; constructor; intuition auto.
-  - constructor; auto. apply IHred1; auto. constructor; simpl; auto.
-  - constructor; auto. induction H; inv H0; constructor; intuition auto.
-  - auto.
-Qed.
-
 Lemma All_local_env_app `{checker_flags} (P : global_context -> context -> term -> term -> Type) Σ l l' :
   All_local_env P Σ (l ,,, l') -> All_local_env P Σ l * All_local_env (fun Σ Γ t T => P Σ (l ,,, Γ) t T) Σ l'.
 Proof.
@@ -1721,35 +1607,6 @@ Proof.
   inv X. eapply localenv_cons_abs. apply IHl'. apply X0. apply X1.
   eapply localenv_cons_def. apply IHl'. apply X0. apply X1.
 Qed.
-
-Definition wf_decl d := match decl_body d with Some b => Ast.wf b | None => True end /\ Ast.wf (decl_type d).
-
-Ltac wf := intuition try (eauto with wf || congruence || solve [constructor]).
-Hint Unfold wf_decl vass vdef : wf.
-Hint Extern 10 => progress simpl : wf.
-Hint Unfold snoc : wf.
-Hint Extern 3 => apply wf_lift || apply wf_subst || apply wf_subst_instance_constr : wf.
-Hint Extern 10 => constructor : wf.
-Hint Resolve Forall_skipn : wf.
-
-Lemma wf_inds mind bodies u : Forall Ast.wf (inds mind u bodies).
-Proof.
-  unfold inds. generalize #|bodies|. induction n. constructor.
-  constructor; auto. wf.
-Qed.
-
-Hint Resolve wf_inds : wf.
-
-Ltac specialize_goal :=
-  repeat match goal with
-  | H : ?P -> _, H' : ?P |- _ => specialize (H H')
-  end.
-
-Definition on_local_decl (P : global_context -> context -> term -> term -> Type) Σ Γ d :=
-  match d.(decl_body) with
-  | Some b => P Σ Γ b d.(decl_type)
-  | None => { u & P Σ Γ d.(decl_type) (tSort u) }
-  end.
 
 Lemma All_local_env_lookup `{checker_flags} {P Σ Γ n} {decl} :
   All_local_env P Σ Γ ->
@@ -1771,147 +1628,10 @@ Proof.
   intuition. destruct a. destruct decl_body.
   inv b. econstructor; eauto. inv b; econstructor; eauto. Qed.
 
-Lemma map_vass_map_def g l n k :
-  (mapi (fun i (d : def term) => vass (dname d) (lift0 i (dtype d)))
-        (map (map_def (lift n k) g) l)) =
-  (mapi (fun i d => map_decl (lift n (i + k)) d) (mapi (fun i (d : def term) => vass (dname d) (lift0 i (dtype d))) l)).
-Proof.
-  rewrite mapi_mapi mapi_map. apply mapi_ext.
-  intros. unfold map_decl, vass; simpl; f_equal.
-  rewrite permute_lift. lia. f_equal; lia.
-Qed.
-
 Lemma All_local_env_map `{checker_flags} (P : global_context -> context -> term -> term -> Type) Σ f l :
   (forall u, f (tSort u) = tSort u) ->
   All_local_env (fun Σ Γ t T => P Σ (map (map_decl f) Γ) (f t) (f T)) Σ l -> All_local_env P Σ (map (map_decl f) l).
 Proof.
   intros Hf. induction 1; econstructor; eauto.
   simpl. rewrite Hf in t0. eapply t0.
-Qed.
-
-Lemma wf_lift_wf n k t : Ast.wf (lift n k t) -> Ast.wf t.
-Proof.
-  induction t in n, k |- * using term_forall_list_ind; simpl in *;
-    intros Hwf; inv Hwf; try constructor; eauto.
-
-  - apply Forall_map_inv in H0. merge_Forall. eapply Forall_impl; eauto.
-    simpl ; intros. intuition eauto.
-  - destruct t; try discriminate. simpl in *. congruence.
-  - destruct l; simpl in *; congruence.
-  - apply Forall_map_inv in H3. merge_Forall. eapply Forall_impl; eauto.
-    simpl ; intros. intuition eauto.
-  - apply Forall_map_inv in H2. merge_Forall. eapply Forall_impl; eauto.
-    simpl ; intros. intuition eauto. unfold compose in *.
-    destruct x; simpl in *; eauto.
-  - apply Forall_map_inv in H0. merge_Forall. eapply Forall_impl; eauto.
-    simpl ; intros. unfold compose in *; destruct x; simpl in *; intuition eauto.
-    destruct dbody; try discriminate. simpl in H5. destruct Nat.leb; auto.
-    reflexivity.
-  - apply Forall_map_inv in H0. merge_Forall. eapply Forall_impl; eauto.
-    simpl ; intros. unfold compose in *; destruct x; simpl in *; intuition eauto.
-Qed.
-
-Lemma typing_wf_gen `{checker_flags} : env_prop (fun Σ Γ t T => Ast.wf t /\ Ast.wf T).
-Proof.
-  apply typing_ind_env; intros; auto with wf;
-    specialize_goal;
-    try solve [split; try constructor; intuition auto with wf].
-
-  - split; wf. apply wf_lift.
-    apply (All_local_env_lookup H1) in H0.
-    red in H0. destruct decl as [na [body|] ty]; simpl in *; intuition auto.
-    destruct H0; intuition auto.
-  - split. constructor; auto. wf.
-    clear H1 H2 X.
-    induction X0. wf. constructor. wf.
-    apply IHX0. split. wf. apply wf_subst. wf. wf. now inv H0.
-    clear H1 H2 X.
-    induction X0. wf. apply IHX0. constructor. wf.
-    apply wf_subst. wf. wf. now inv H0.
-  - split. wf. apply wf_subst_instance_constr. wf.
-    red in H0.
-    eapply lookup_on_global_env in H0 as [Σ' [wfΣ' prf]]; eauto.
-    red in prf. destruct decl; destruct cst_body; red in prf; simpl in *; wf.
-    destruct prf. apply a.
-
-  - split. wf. apply wf_subst_instance_constr. wf.
-    destruct isdecl as [Hmdecl Hidecl]. red in Hmdecl.
-    eapply lookup_on_global_env in X as [Σ' [wfΣ' prf]]; eauto.
-    apply onInductives in prf.
-    eapply nth_error_alli in Hidecl; eauto.
-    eapply onArity in Hidecl.
-    destruct Hidecl as [[s Hs] Hpars]; wf.
-  - split. wf.
-    destruct isdecl as [[Hmdecl Hidecl] Hcdecl]. red in Hmdecl.
-    eapply lookup_on_global_env in X as [Σ' [wfΣ' prf]]; eauto. red in prf.
-    apply onInductives in prf.
-    eapply nth_error_alli in Hidecl; eauto. simpl in *. intuition.
-    apply onConstructors in Hidecl.
-    eapply nth_error_alli in Hcdecl; eauto.
-    destruct Hcdecl as [[s Hs] Hpars]. unfold type_of_constructor. wf.
-  - split. wf. constructor; eauto.
-    eapply Forall2_Forall_left; eauto. simpl. intuition auto.
-    apply wf_mkApps. wf. apply Forall_app_inv. split. 2:wf.
-    inv H6. apply wf_mkApps_inv in H8. now apply Forall_skipn.
-  - split. wf. apply wf_subst. constructor. wf. intuition.
-    apply wf_mkApps_inv in H3. now apply Forall_rev.
-    subst ty. destruct isdecl as [[Hmdecl Hidecl] Hpdecl].
-    eapply lookup_on_global_env in Hmdecl as [Σ' [wfΣ' prf]]; eauto. red in prf.
-    apply onInductives in prf.
-    eapply nth_error_alli in Hidecl; eauto. intuition.
-    eapply onProjections in Hidecl.
-    eapply nth_error_alli in Hidecl; eauto. red in Hidecl.
-    destruct decompose_prod_assum.
-    destruct Hidecl as [[s Hs] Hnpars]. apply wf_subst_instance_constr. apply Hs.
-  - subst types.
-    apply All_local_env_app in X as [HΓ Hmfix].
-    clear Hmfix.
-    split.
-    + revert X0. generalize (fix_context mfix). intros.
-      clear decl H0. constructor. induction mfix. constructor. constructor.
-      2:{ apply IHmfix. inv X0. auto. }
-      inv X0. intuition. now apply wf_lift_wf in H1.
-    + eapply nth_error_all in X0; eauto. simpl in X0. intuition eauto.
-      now apply wf_lift_wf in H2.
-  - subst types.
-    apply All_local_env_app in X as [HΓ Hmfix].
-    clear Hmfix.
-    split.
-    + revert X0. generalize (fix_context mfix). intros.
-      clear decl H0. constructor. induction mfix. constructor. constructor.
-      2:{ apply IHmfix. inv X0. auto. }
-      inv X0. intuition. now apply wf_lift_wf in H1.
-    + eapply nth_error_all in X0; eauto. simpl in X0; intuition eauto.
-      now apply wf_lift_wf in H2.
-Qed.
-
-Lemma typing_all_wf_decl `{checker_flags} Σ (wfΣ : wf Σ) Γ (wfΓ : wf_local Σ Γ) :
-  Forall wf_decl Γ.
-Proof.
-  induction wfΓ. constructor. constructor; auto. red. simpl. split; wf.
-  apply typing_wf_gen in t0; eauto. apply t0; auto.
-  constructor; auto. red; simpl. apply typing_wf_gen in t0; auto. intuition auto.
-Qed.
-Hint Resolve typing_all_wf_decl : wf.
-
-Lemma typing_wf_sigma `{checker_flags} Σ (wfΣ : wf Σ) :
-  on_global_env (fun Σ Γ t T => match t with Some b => Ast.wf b /\ Ast.wf T | None => Ast.wf T end) Σ.
-Proof.
-  intros.
-  pose proof (env_prop_sigma _ typing_wf_gen _ wfΣ). red in X.
-  red in X. unfold lift_typing in X. red. do 2 red in wfΣ.
-  unshelve eapply (on_global_decls_mix _ wfΣ) in X.
-  red. intros. destruct b; intuition auto with wf.
-  destruct X0 as [u Hu]. exists u. intuition auto with wf.
-  clear wfΣ.
-  eapply on_global_decls_impl; eauto; simpl; intros. clear X.
-  destruct X1 as [Hty Ht].
-  pose proof (on_global_decls_proj X0).
-  destruct t. apply Ht. destruct Ht; wf.
-Qed.
-
-Lemma typing_wf `{checker_flags} Σ (wfΣ : wf Σ) Γ t T :
-  Σ ;;; Γ |- t : T -> Ast.wf t /\ Ast.wf T.
-Proof.
-  intros. eapply typing_wf_gen in X; intuition eauto with wf.
 Qed.
