template-coq/theories/Generation.v
@@ -1,0 +1,57 @@
+(* Distributed under the terms of the MIT license.   *)
+
+From Coq Require Import Bool String List Program BinPos Compare_dec Omega Lia.
+From Template Require Import config utils Ast AstUtils Induction utils LiftSubst UnivSubst Typing.
+Require Import ssreflect ssrbool.
+
+(** * Substitution lemmas for typing derivations. *)
+
+Set Asymmetric Patterns.
+Close Scope string_scope.
+
+Lemma invert_type_App `{checker_flags} Σ Γ f u T :
+  Σ ;;; Γ |- tApp f u : T ->
+  { T' : term & { U' & ((Σ ;;; Γ |- f : T') * typing_spine Σ Γ T' u U' *
+                        (isApp f <> true) * (u <> []) *
+                        (Σ ;;; Γ |- U' <= T))%type } }.
+Proof.
+  intros Hty.
+  dependent induction Hty.
+  exists t_ty, t'. intuition.
+  specialize (IHHty1 _ _ eq_refl) as [T' [U' [H' H'']]].
+  exists T', U'. split; auto.
+  eapply cumul_trans; eauto.
+Qed.
+
+Lemma type_mkApp `{checker_flags} Σ Γ f u T T' :
+  Σ ;;; Γ |- f : T ->
+  typing_spine Σ Γ T [u] T' ->
+  Σ ;;; Γ |- mkApp f u : T'.
+Proof.
+  intros Hf Hu. inv Hu.
+  simpl. destruct (isApp f) eqn:Happ.
+  destruct f; try discriminate. simpl.
+  eapply invert_type_App in Hf.
+  destruct Hf as (T'' & U' & (((Hf & HU) & Happf) & Hunil) & Hcumul).
+  eapply type_App; eauto. intro. apply Hunil.
+  destruct l; simpl in *; congruence.
+  inv X1. clear Happ Hf Hunil.
+  induction HU. simpl. econstructor; eauto.
+  eapply cumul_trans; eauto.
+  econstructor. econstructor. eapply t. eauto. eauto.
+  apply IHHU; eauto.
+  rewrite -> mkApp_tApp; eauto.
+  econstructor; eauto. congruence.
+  econstructor; eauto.
+Qed.
+
+Lemma type_mkApps `{checker_flags} Σ Γ f u T T' :
+  Σ ;;; Γ |- f : T ->
+  typing_spine Σ Γ T u T' ->
+  Σ ;;; Γ |- mkApps f u : T'.
+Proof.
+  intros Hf Hu. induction Hu in f, Hf |- *. auto.
+  rewrite <- mkApps_mkApp.
+  eapply IHHu. eapply type_mkApp. eauto.
+  econstructor; eauto. constructor.
+Qed.
