template-coq/theories/TypingWf.v
@@ -1,0 +1,336 @@
+(* Distributed under the terms of the MIT license.   *)
+
+From Coq Require Import Bool String List Program BinPos Compare_dec Arith Lia.
+From Template Require Import config utils Ast AstUtils univ Induction LiftSubst UnivSubst Typing.
+Require Import ssreflect.
+
+Set Asymmetric Patterns.
+
+(** * Well-formedness of terms and types in typing derivations
+
+  The internal representation of terms is not canonical, so we show
+  that only well-formed terms and types can appear in typing derivations
+  and the global context.
+*)
+
+
+Definition wf_decl d := match decl_body d with Some b => Ast.wf b | None => True end /\ Ast.wf (decl_type d).
+
+Definition wf_decl_pred : global_context -> context -> term -> term -> Type :=
+  (fun _ _ t T => Ast.wf t /\ Ast.wf T).
+
+Lemma All_local_env_wf_decl:
+  forall Σ (Γ : context),
+    Forall wf_decl Γ -> All_local_env wf_decl_pred Σ Γ.
+Proof.
+  intros Σ Γ X.
+  induction Γ in X |- *.
+  - constructor; eauto.
+  - destruct a as [na [body|] ty].
+    constructor. apply IHΓ. inv X; eauto.
+    red. inv X. eauto.
+    eapply (localenv_cons_abs _ _ _ _ _ (Universe.make Level.lProp)).
+    apply IHΓ. inv X; eauto.
+    red. inv X. red in H. intuition eauto. constructor.
+Qed.
+
+Lemma All_local_env_wf_decl_inv:
+  forall (Σ : global_context) (a : context_decl) (Γ : list context_decl)
+         (X : All_local_env wf_decl_pred Σ (a :: Γ)),
+    on_local_decl wf_decl_pred Σ Γ a * All_local_env wf_decl_pred Σ Γ.
+Proof.
+  intros Σ a Γ X.
+  inv X; intuition; red; simpl; eauto.
+Qed.
+
+Lemma wf_strip_outer_cast t : Ast.wf t -> Ast.wf (strip_outer_cast t).
+Proof.
+  induction t; auto.
+  simpl. intros H; now inv H.
+Qed.
+
+Lemma wf_mkApps_napp t u : isApp t = false -> Ast.wf (mkApps t u) -> Ast.wf t /\ List.Forall Ast.wf u.
+Proof.
+  induction u in t |- *; simpl.
+  - intuition.
+  - intros Happ H; destruct t; try solve [inv H; intuition auto].
+    specialize (IHu (tApp t (l ++ [a]))).
+    forward IHu.
+    induction u; trivial. discriminate.
+Qed.
+Hint Resolve wf_mkApps_napp : wf.
+
+Lemma wf_mkApps_inv t u : Ast.wf (mkApps t u) -> List.Forall Ast.wf u.
+Proof.
+  induction u in t |- *; simpl.
+  - intuition.
+  - intros H; destruct t; try solve [inv H; intuition auto].
+    specialize (IHu (tApp t (l ++ [a]))).
+    forward IHu.
+    induction u; trivial.
+    simpl. rewrite <- app_assoc. simpl. apply H.
+    intuition. inv H.
+    apply Forall_app in H3. intuition.
+Qed.
+Hint Resolve wf_mkApps_inv : wf.
+Hint Constructors Ast.wf : wf.
+
+Lemma isLambda_isApp t : isLambda t = true -> isApp t = false.
+Proof. destruct t; simpl; congruence. Qed.
+
+Lemma unfold_fix_wf:
+  forall (mfix : mfixpoint term) (idx : nat) (narg : nat) (fn : term),
+    unfold_fix mfix idx = Some (narg, fn) ->
+    Ast.wf (tFix mfix idx) ->
+    Ast.wf fn /\ isApp fn <> true.
+Proof.
+  intros mfix idx narg fn Hf Hwf.
+  unfold unfold_fix in Hf. inv Hwf.
+  destruct nth_error eqn:eqnth; try congruence.
+  pose proof (nth_error_forall eqnth H). simpl in H0.
+  injection Hf. intros <- <-.
+  destruct H0 as [ _ [ wfd islamd ] ]. apply (isLambda_subst (fix_subst mfix) 0) in islamd.
+  apply isLambda_isApp in islamd. split; try congruence.
+  apply wf_subst; auto. clear wfd islamd Hf eqnth.
+  assert(forall n, Ast.wf (tFix mfix n)). constructor; auto.
+  unfold fix_subst. generalize #|mfix|; intros. induction n; auto.
+Qed.
+
+Lemma unfold_cofix_wf:
+  forall (mfix : mfixpoint term) (idx : nat) (narg : nat) (fn : term),
+    unfold_cofix mfix idx = Some (narg, fn) ->
+    Ast.wf (tCoFix mfix idx) -> Ast.wf fn.
+Proof.
+  intros mfix idx narg fn Hf Hwf.
+  unfold unfold_cofix in Hf. inv Hwf.
+  destruct nth_error eqn:eqnth; try congruence.
+  pose proof (nth_error_forall eqnth H). simpl in H0.
+  injection Hf. intros <- <-.
+  destruct H0 as [ _ wfd ].
+  apply wf_subst; auto. clear wfd Hf eqnth.
+  assert(forall n, Ast.wf (tCoFix mfix n)). constructor; auto.
+  unfold cofix_subst. generalize #|mfix|; intros. induction n; auto.
+Qed.
+
+Lemma wf_subst_instance_constr u c :
+  Ast.wf c -> Ast.wf (subst_instance_constr u c).
+Proof.
+  induction 1 using term_wf_forall_list_ind; simpl; try solve [ constructor; auto using Forall_map ].
+
+  constructor; auto. destruct t; simpl in *; try congruence. destruct l; simpl in *; congruence.
+  now apply Forall_map.
+  constructor; auto. merge_Forall. apply Forall_map.
+  eapply Forall_impl; eauto. intros. simpl in *. red. intuition auto.
+  destruct x; simpl in *.
+  destruct dbody; simpl in *; congruence.
+Qed.
+
+Lemma wf_nth:
+  forall (n : nat) (args : list term), Forall Ast.wf args -> Ast.wf (nth n args tDummy).
+Proof.
+  intros n args H. induction H in n; destruct n; simpl; try constructor; auto.
+Qed.
+Hint Resolve wf_nth.
+
+Lemma wf_red1 `{CF:checker_flags} Σ Γ M N :
+  on_global_env (fun Σ Γ t T => match t with Some b => Ast.wf b /\ Ast.wf T | None => Ast.wf T end) Σ ->
+  List.Forall (fun d => match decl_body d with Some b => Ast.wf b | None => True end) Γ ->
+  Ast.wf M -> red1 (fst Σ) Γ M N -> Ast.wf N.
+Proof.
+  intros wfΣ wfΓ wfM H.
+  induction H using red1_ind_all in wfM, wfΓ |- *; inv wfM; try solve[ constructor; auto with wf ].
+
+  - inv H1. inv H2.
+    eauto with wf.
+  - auto with wf.
+  - apply wf_lift.
+    unfold option_map in H. destruct nth_error eqn:Heq; try discriminate.
+    eapply nth_error_forall in wfΓ; eauto. simpl in *. destruct (decl_body c); congruence.
+  - unfold iota_red.
+    apply wf_mkApps_inv in H0.
+    apply wf_mkApps; auto.
+    induction brs in c, H1 |- *; destruct c; simpl in *. constructor. constructor.
+    inv H1; auto. inv H1; auto.
+    induction H0 in pars |- *; destruct pars; try constructor; auto. simpl. auto.
+  - apply unfold_fix_wf in H; auto. constructor; intuition auto.
+  - constructor; auto. apply wf_mkApps_napp in H1 as [Hcof Hargs]; auto.
+    apply unfold_cofix_wf in H; auto.
+    apply wf_mkApps; intuition auto.
+  - constructor; auto. apply wf_mkApps_napp in H0 as [Hcof Hargs]; auto.
+    apply unfold_cofix_wf in H; auto.
+    apply wf_mkApps; intuition auto.
+  - apply wf_subst_instance_constr.
+    unfold declared_constant in H.
+    eapply lookup_on_global_env in H as [Σ' [onΣ' prf]]; eauto.
+    destruct decl; simpl in *.
+    subst cst_body; intuition. red in prf. simpl in prf. easy.
+  - apply wf_mkApps_inv in H0.
+    eapply nth_error_forall in H0; eauto.
+  - constructor; auto. apply IHred1; auto. constructor; simpl; auto.
+  - constructor; auto. apply IHred1; auto. constructor; simpl; auto.
+  - constructor; auto. induction H; constructor; inv H2; intuition auto.
+  - apply wf_mkApps; auto.
+  - constructor; auto. induction H; congruence.
+    clear H1. induction H; inv H3; constructor; intuition auto.
+  - constructor; auto. apply IHred1; auto. constructor; simpl; auto.
+  - constructor; auto. induction H; inv H0; constructor; intuition auto.
+  - auto.
+Qed.
+
+Ltac wf := intuition try (eauto with wf || congruence || solve [constructor]).
+Hint Unfold wf_decl vass vdef : wf.
+Hint Extern 10 => progress simpl : wf.
+Hint Unfold snoc : wf.
+Hint Extern 3 => apply wf_lift || apply wf_subst || apply wf_subst_instance_constr : wf.
+Hint Extern 10 => constructor : wf.
+Hint Resolve Forall_skipn : wf.
+
+Lemma wf_inds mind bodies u : Forall Ast.wf (inds mind u bodies).
+Proof.
+  unfold inds. generalize #|bodies|. induction n. constructor.
+  constructor; auto. wf.
+Qed.
+
+Hint Resolve wf_inds : wf.
+
+Ltac specialize_goal :=
+  repeat match goal with
+  | H : ?P -> _, H' : ?P |- _ => specialize (H H')
+  end.
+
+Lemma map_vass_map_def g l n k :
+  (mapi (fun i (d : def term) => vass (dname d) (lift0 i (dtype d)))
+        (map (map_def (lift n k) g) l)) =
+  (mapi (fun i d => map_decl (lift n (i + k)) d) (mapi (fun i (d : def term) => vass (dname d) (lift0 i (dtype d))) l)).
+Proof.
+  rewrite mapi_mapi mapi_map. apply mapi_ext.
+  intros. unfold map_decl, vass; simpl; f_equal.
+  rewrite permute_lift. lia. f_equal; lia.
+Qed.
+
+Lemma wf_lift_wf n k t : Ast.wf (lift n k t) -> Ast.wf t.
+Proof.
+  induction t in n, k |- * using term_forall_list_ind; simpl in *;
+    intros Hwf; inv Hwf; try constructor; eauto.
+
+  - apply Forall_map_inv in H0. merge_Forall. eapply Forall_impl; eauto.
+    simpl ; intros. intuition eauto.
+  - destruct t; try discriminate. simpl in *. congruence.
+  - destruct l; simpl in *; congruence.
+  - apply Forall_map_inv in H3. merge_Forall. eapply Forall_impl; eauto.
+    simpl ; intros. intuition eauto.
+  - apply Forall_map_inv in H2. merge_Forall. eapply Forall_impl; eauto.
+    simpl ; intros. intuition eauto. unfold compose in *.
+    destruct x; simpl in *; eauto.
+  - apply Forall_map_inv in H0. merge_Forall. eapply Forall_impl; eauto.
+    simpl ; intros. unfold compose in *; destruct x; simpl in *; intuition eauto.
+    destruct dbody; try discriminate. simpl in H5. destruct Nat.leb; auto.
+    reflexivity.
+  - apply Forall_map_inv in H0. merge_Forall. eapply Forall_impl; eauto.
+    simpl ; intros. unfold compose in *; destruct x; simpl in *; intuition eauto.
+Qed.
+
+Lemma typing_wf_gen `{checker_flags} : env_prop (fun Σ Γ t T => Ast.wf t /\ Ast.wf T).
+Proof.
+  apply typing_ind_env; intros; auto with wf;
+    specialize_goal;
+    try solve [split; try constructor; intuition auto with wf].
+
+  - split; wf. apply wf_lift.
+    apply (All_local_env_lookup H1) in H0.
+    red in H0. destruct decl as [na [body|] ty]; simpl in *; intuition auto.
+    destruct H0; intuition auto.
+  - split. constructor; auto. wf.
+    clear H1 H2 X.
+    induction X0. wf. constructor. wf.
+    apply IHX0. split. wf. apply wf_subst. wf. wf. now inv H0.
+    clear H1 H2 X.
+    induction X0. wf. apply IHX0. constructor. wf.
+    apply wf_subst. wf. wf. now inv H0.
+  - split. wf. apply wf_subst_instance_constr. wf.
+    red in H0.
+    eapply lookup_on_global_env in H0 as [Σ' [wfΣ' prf]]; eauto.
+    red in prf. destruct decl; destruct cst_body; red in prf; simpl in *; wf.
+    destruct prf. apply a.
+
+  - split. wf. apply wf_subst_instance_constr. wf.
+    destruct isdecl as [Hmdecl Hidecl]. red in Hmdecl.
+    eapply lookup_on_global_env in X as [Σ' [wfΣ' prf]]; eauto.
+    apply onInductives in prf.
+    eapply nth_error_alli in Hidecl; eauto.
+    eapply onArity in Hidecl.
+    destruct Hidecl as [[s Hs] Hpars]; wf.
+  - split. wf.
+    destruct isdecl as [[Hmdecl Hidecl] Hcdecl]. red in Hmdecl.
+    eapply lookup_on_global_env in X as [Σ' [wfΣ' prf]]; eauto. red in prf.
+    apply onInductives in prf.
+    eapply nth_error_alli in Hidecl; eauto. simpl in *. intuition.
+    apply onConstructors in Hidecl.
+    eapply nth_error_alli in Hcdecl; eauto.
+    destruct Hcdecl as [[s Hs] Hpars]. unfold type_of_constructor. wf.
+  - split. wf. constructor; eauto.
+    eapply Forall2_Forall_left; eauto. simpl. intuition auto.
+    apply wf_mkApps. wf. apply Forall_app_inv. split. 2:wf.
+    inv H6. apply wf_mkApps_inv in H8. now apply Forall_skipn.
+  - split. wf. apply wf_subst. constructor. wf. intuition.
+    apply wf_mkApps_inv in H3. now apply Forall_rev.
+    subst ty. destruct isdecl as [[Hmdecl Hidecl] Hpdecl].
+    eapply lookup_on_global_env in Hmdecl as [Σ' [wfΣ' prf]]; eauto. red in prf.
+    apply onInductives in prf.
+    eapply nth_error_alli in Hidecl; eauto. intuition.
+    eapply onProjections in Hidecl.
+    eapply nth_error_alli in Hidecl; eauto. red in Hidecl.
+    destruct decompose_prod_assum.
+    destruct Hidecl as [[s Hs] Hnpars]. apply wf_subst_instance_constr. apply Hs.
+  - subst types.
+    apply All_local_env_app in X as [HΓ Hmfix].
+    clear Hmfix.
+    split.
+    + revert X0. generalize (fix_context mfix). intros.
+      clear decl H0. constructor. induction mfix. constructor. constructor.
+      2:{ apply IHmfix. inv X0. auto. }
+      inv X0. intuition. now apply wf_lift_wf in H1.
+    + eapply nth_error_all in X0; eauto. simpl in X0. intuition eauto.
+      now apply wf_lift_wf in H2.
+  - subst types.
+    apply All_local_env_app in X as [HΓ Hmfix].
+    clear Hmfix.
+    split.
+    + revert X0. generalize (fix_context mfix). intros.
+      clear decl H0. constructor. induction mfix. constructor. constructor.
+      2:{ apply IHmfix. inv X0. auto. }
+      inv X0. intuition. now apply wf_lift_wf in H1.
+    + eapply nth_error_all in X0; eauto. simpl in X0; intuition eauto.
+      now apply wf_lift_wf in H2.
+Qed.
+
+Lemma typing_all_wf_decl `{checker_flags} Σ (wfΣ : wf Σ) Γ (wfΓ : wf_local Σ Γ) :
+  Forall wf_decl Γ.
+Proof.
+  induction wfΓ. constructor. constructor; auto. red. simpl. split; wf.
+  apply typing_wf_gen in t0; eauto. apply t0; auto.
+  constructor; auto. red; simpl. apply typing_wf_gen in t0; auto. intuition auto.
+Qed.
+Hint Resolve typing_all_wf_decl : wf.
+
+Lemma typing_wf_sigma `{checker_flags} Σ (wfΣ : wf Σ) :
+  on_global_env (fun Σ Γ t T => match t with Some b => Ast.wf b /\ Ast.wf T | None => Ast.wf T end) Σ.
+Proof.
+  intros.
+  pose proof (env_prop_sigma _ typing_wf_gen _ wfΣ). red in X.
+  red in X. unfold lift_typing in X. red. do 2 red in wfΣ.
+  unshelve eapply (on_global_decls_mix _ wfΣ) in X.
+  red. intros. destruct b; intuition auto with wf.
+  destruct X0 as [u Hu]. exists u. intuition auto with wf.
+  clear wfΣ.
+  eapply on_global_decls_impl; eauto; simpl; intros. clear X.
+  destruct X1 as [Hty Ht].
+  pose proof (on_global_decls_proj X0).
+  destruct t. apply Ht. destruct Ht; wf.
+Qed.
+
+Lemma typing_wf `{checker_flags} Σ (wfΣ : wf Σ) Γ t T :
+  Σ ;;; Γ |- t : T -> Ast.wf t /\ Ast.wf T.
+Proof.
+  intros. eapply typing_wf_gen in X; intuition eauto with wf.
+Qed.
