template-coq/theories/Weakening.v
@@ -1,7 +1,7 @@
 (* Distributed under the terms of the MIT license.   *)
 
 From Coq Require Import Bool String List Program BinPos Compare_dec Omega Lia.
-From Template Require Import config utils Ast AstUtils Induction utils LiftSubst Typing.
+From Template Require Import config utils Ast AstUtils Induction utils LiftSubst Typing TypingWf.
 From Template Require Import WeakeningEnv Closed.
 
 (** * Weakening lemmas for typing derivations.
